core/ProofMonads.v
@@ -1,4 +1,4 @@
-Require Import Program Monads.
+Require Import Program Monads Omega ZArith.
 
 Set Implicit Arguments.
 
@@ -22,24 +22,24 @@ Lemma bind_eq : forall {A B m} `{Monad m} (a a' : m A) (f f' : A -> m B),
 
 Section state_proof.
 
-Variable S : Type.
+Variable St : Type.
 
-Definition State := M.State S.
+Definition State := M.State St.
 
 Check State.
 
-Definition hoareTripleS {A} (P : S -> Prop) (m : State A) (Q : A -> S -> Prop) : Prop :=
-  forall (s : S), P s -> let (a, s') := m s in Q a s'.
+Definition hoareTripleS {A} (P : St -> Prop) (m : State A) (Q : A -> St -> Prop) : Prop :=
+  forall (s : St), P s -> let (a, s') := m s in Q a s'.
 
 Notation "{{ P }} m {{ Q }}" := (hoareTripleS P m Q)
   (at level 90, format "'[' '[' {{  P  }}  ']' '/  ' '[' m ']' '['  {{  Q  }} ']' ']'") : monad_scope.
 
-Lemma ret (A : Type) `{State A} (a : A) (P : A -> S -> Prop) : {{ P a }} return_ a {{ P }}.
+Lemma ret (A : Type) `{State A} (a : A) (P : A -> St -> Prop) : {{ P a }} return_ a {{ P }}.
 Proof.
 intros s H; trivial.
 Qed.
 
-Lemma bind (A B : Type) (m : State A) (f : A -> State B) (P : S -> Prop)( Q : A -> S -> Prop) (R : B -> S -> Prop) :
+Lemma bind (A B : Type) (m : State A) (f : A -> State B) (P : St -> Prop)( Q : A -> St -> Prop) (R : B -> St -> Prop) :
   (forall a, {{ Q a }} f a {{ R }}) -> {{ P }} m {{ Q }} -> {{ P }} perf x <- m ; f x {{ R }}.
 Proof.
 intros H1 H2 s Hs.
@@ -57,10 +57,10 @@ rewrite H5 in Hs.
 trivial.
 Qed.
 
-Definition wp {A : Type} (P : A -> S -> Prop) (m : State A) :=
+Definition wp {A : Type} (P : A -> St -> Prop) (m : State A) :=
   fun s => let (a,s') := m s in P a s'.
 
-Lemma wpIsPrecondition {A : Type} (P : A -> S -> Prop) (m : State A) :
+Lemma wpIsPrecondition {A : Type} (P : A -> St -> Prop) (m : State A) :
   {{ wp P m }} m {{ P }}.
   Proof.
   unfold wp.
@@ -68,7 +68,7 @@ Lemma wpIsPrecondition {A : Type} (P : A -> S -> Prop) (m : State A) :
   Qed.
 
 Lemma wpIsWeakestPrecondition
-  (A : Type) (P : A -> S -> Prop) (Q : S -> Prop) (m : State A) :
+  (A : Type) (P : A -> St -> Prop) (Q : St -> Prop) (m : State A) :
   {{ Q }} m {{ P }} -> forall s, Q s -> (wp P m) s.
   Proof.
   trivial.
@@ -94,23 +94,23 @@ Lemma assoc (A B C : Type)(m : State A)(f : A -> State B)(g : B -> State C) :
   reflexivity.
   Qed.
 
-Lemma put (s : S) (P : unit -> S -> Prop) : {{ fun _ => P tt s }} putS s {{ P }}.
+Lemma put (s : St) (P : unit -> St -> Prop) : {{ fun _ => P tt s }} putS s {{ P }}.
 Proof.
 intros s0 H;trivial.
 Qed.
 
-Lemma get (P : S -> S -> Prop) : {{ fun s => P s s }} @getS S {{ P }}.
+Lemma get (P : St -> St -> Prop) : {{ fun s => P s s }} @getS St {{ P }}.
 Proof.
 intros s H; trivial.
 Qed.
 
-Lemma sequence_rule (A B : Type) (m : State A) (f : A -> State B) (P : S -> Prop)( Q : A -> S -> Prop) (R : B -> S -> Prop) :
+Lemma sequence_rule (A B : Type) (m : State A) (f : A -> State B) (P : St -> Prop)( Q : A -> St -> Prop) (R : B -> St -> Prop) :
   {{ P }} m {{ Q }} -> (forall a, {{ Q a }} f a {{ R }}) -> {{ P }} perf x <- m ; f x {{ R }}.
 Proof.
 intros; eapply bind ; eassumption.
 Qed.
 
-Lemma weaken (A : Type) (m : State A) (P Q : S -> Prop) (R : A -> S -> Prop) :
+Lemma weaken (A : Type) (m : State A) (P Q : St -> Prop) (R : A -> St -> Prop) :
   {{ Q }} m {{ R }} -> (forall s, P s -> Q s) -> {{ P }} m {{ R }}.
 Proof.
 intros H1 H2 s H3.
@@ -119,7 +119,7 @@ apply H1 in H3.
 assumption.
 Qed.
 
-Lemma modify f (P : () -> S -> Prop) : {{ fun s => P tt (f s) }} modify f {{ P }}.
+Lemma modify f (P : () -> St -> Prop) : {{ fun s => P tt (f s) }} modify f {{ P }}.
 Proof.
 unfold modify.
 eapply bind.
@@ -132,7 +132,76 @@ intros. simpl.
 assumption.
 Qed.
 
-End state_proof.
+Lemma act_ret  (A : Type) (a : A) (P : St -> Prop) : {{P}} state_pure (Atom a) 
+{{fun (_ : Action A) =>  P }}.
+Proof.
+intros s H; trivial.
+Qed.
 
-Notation "{{ P }} m {{ Q }}" := (hoareTripleS P m Q)
-  (at level 90, format "'[' '[' {{  P  }}  ']' '/  ' '[' m ']' '['  {{  Q  }} ']' ']'") : monad_scope.
+Lemma foreach_rule (min max : nat) (P : nat -> St -> Prop) (body : nat -> State () ):
+  (forall (it : nat), {{fun s => P it s /\ (min < it <= max)}} body it {{fun _ => P (it - 1)}}) /\  min <= max ->
+    {{P max}} M.foreach2_st max min (fun it0 => loopeT_liftT (body it0)) {{fun _ => P min}}.
+    Proof.
+    intros [Hleq Hmaxmin].
+    induction max.
+     + assert (min = 0) by omega.
+      replace min with 0.
+      intros s Hs.
+      simpl.
+      auto.
+    + unfold M.foreach2_st.
+      case_eq (S max <=? min);intros Hm.
+      - intros s HP.
+        cbn.
+        rewrite Nat.leb_le in Hm.
+        assert (S max = min) by omega.
+        rewrite H in HP.
+        auto.
+      - eapply sequence_rule.
+        unfold runLoopeT.
+        unfold loopeT_liftT.
+        unfold liftM.
+        eapply sequence_rule.
+(*         unfold hoareTripleS in Hleq.
+          unfold hoareTriple. *)
+          intros st H2.
+          generalize (Hleq (S max)).
+          intros Hmax.
+          eapply Hmax;split; auto.
+          rewrite Nat.leb_nle in Hm. omega.
+        intros [].
+          apply act_ret.
+      * intros. cbn.
+        replace (max - 0) with (max) by omega.
+        apply IHmax.
+         ++ intros it s'.
+            intros [H1 [H2 H3]].
+            apply Hleq.
+            split;auto.
+        ++ rewrite Nat.leb_nle in Hm.
+           omega.
+       Qed.
+
+Open Scope Z.
+
+Lemma foreach_ruleZ (min max : Z) (P : Z -> St -> Prop) (body : Z -> State () ):
+  0 <= min <= max /\ (forall (it : Z), {{fun s => P it s /\ (min < it <= max)}} body it {{fun _ => P (it + 1)}})  ->
+    {{P min}} M.foreach3_st min max (fun it0 => loopeT_liftT (body it0)) {{fun _ => P max}}.
+    Proof.
+    intros [Hleq Hmaxmin].
+    induction max.
+    + assert (min = 0) by omega.
+      replace min with 0.
+      intros s Hs.
+      simpl.
+      auto.
+    + unfold M.foreach3_st.
+      unfold M.foreach3_st_func.
+      case_eq (Z.pos p <=? min);intros Hm.
+
+(* Lemma foreach3_rule (min max : Z) (P : Z -> St -> Prop) (body : Z -> State ())
+  : (forall (it : Z), 
+    {{fun s => P it s /\ (min < it <= max)}} 
+      body it 
+      {{fun _ => P (it - 1)}}) /\  min <= max ->
+    {{P min}} M.foreach3 min max (fun it0 => loopT_liftT (body it0)) {{fun _ => P max}}. *)
